\documentclass{ximera}
\usepackage{sagetex}
%% handout
%% space
%% newpage
%% numbers
%% nooutcomes

\input{../preamble} %% we can turn off input when making a master document

\outcome{}
\author{Darryl Chamberlain Jr.}
 
\title{Objective 4 - Solve Exponential}

\begin{document}
\begin{abstract}
Solve exponential equations with the same or different bases.
\end{abstract}
\maketitle

\href{https://cnx.org/contents/mwjClAV_@8.1:wfhkHyEh@11/Exponential-and-Logarithmic-Equations}{Link to section in online textbook.}

%%%%%%%%%%%%%%%%%%%%%
%%%  Objective 2  %%%
%%%%%%%%%%%%%%%%%%%%%

Watch the video below to learn how to solve \textbf{any} type of exponential equation. You can print out \href{http://people.clas.ufl.edu/dchamberlain31/files/Objective-4-Solve-Exponential-Equalities.pdf}{these notes} to follow along and keep notes to organize your thoughts.  

\youtube{dR7GkfE9z7E}

\textit{Note: Yes, you can use this method all of the time! While changing the bases to be the same to rewrite the question can be easier sometimes, taking the log of both sides will \textbf{always} solve exponential equations.}

\begin{sagesilent}
x = var("x")

def maybeMakeNegative(natural):
    integer = natural*(-1)**ZZ.random_element(2)
    return integer 

def generateFactor():
    a0 = maybeMakeNegative(ZZ.random_element(2, 7))
    a1 = maybeMakeNegative(ZZ.random_element(2, 7))
    factor = a0*x + a1
    return factor 

#####
factor5a = generateFactor()
factor5b = generateFactor()
base5 = ZZ.random_element(2, 7)
#
while len(solve(factor5a - factor5b == 0, x)) == 0:
    factor5a = generateFactor()
    factor5b = generateFactor()
    base5 = ZZ.random_element(2, 7)
#
solution5 = round(float( solve(factor5a - factor5b == 0, x)[0].rhs() ), 3)
#####
#####
factor6a = generateFactor()
factor6b = generateFactor()
preBase6 = ZZ.random_element(2, 7)
k6 = ZZ.random_element(2, 4)
base6a = preBase6**k6
base6b = preBase6
#
while len(solve(k6*factor6a - factor6b == 0, x)) == 0:
    factor6a = generateFactor()
    factor6b = generateFactor()
    preBase6 = ZZ.random_element(2, 7)
    k6 = ZZ.random_element(2, 4)
    base6a = preBase6**k6
    base6b = preBase6
#
solution6 = round(float( solve(k6*factor6a - factor6b == 0, x)[0].rhs() ), 3)
#####
#####
factor7a = generateFactor()
factor7b = generateFactor()
preBase7 = ZZ.random_element(2, 7)
k7 = -ZZ.random_element(2, 4)
base7a = preBase7**k7
base7b = preBase7
#
while len(solve(k7*factor7a - factor7b == 0, x)) == 0:
    factor7a = generateFactor()
    factor7b = generateFactor()
    preBase7 = ZZ.random_element(2, 7)
    k7 = -ZZ.random_element(2, 4)
    base7a = preBase7**k7
    base7b = preBase7
#
solution7 = round(float( solve(k7*factor7a - factor7b == 0, x)[0].rhs() ), 3)
#####
#####
factor8a = generateFactor()
factor8b = generateFactor()
preBase8 = ZZ.random_element(2, 7)
k8a = ZZ.random_element(2, 4)
k8b = k8a + ZZ.random_element(1, 2)
base8a = preBase8**k8a
base8b = preBase8**k8b
#
while len(solve(k8a*factor8a - k8b*factor8b == 0, x)) == 0:
    factor8a = generateFactor()
    factor8b = generateFactor()
    preBase8 = ZZ.random_element(2, 7)
    k8a = ZZ.random_element(2, 4)
    k8b = k8a + ZZ.random_element(1, 2)
    base8a = preBase8**k8a
    base8b = preBase8**k8b
#
solution8 = round(float( solve(k8a*factor8a - k8b*factor8b == 0, x)[0].rhs() ), 3)
\end{sagesilent}

% Q5
\begin{question}
Solve the exponential equation below.

$$ \sage{base5}^{\sage{factor5a}} = \sage{base5}^{\sage{factor5b}} $$

$ x = \answer[tolerance=0.05]{\sage{solution5}} $
\end{question}

% Q6
\begin{question}
Solve the exponential equation below. 

$$ \sage{base6a}^{\sage{factor6a}} = \sage{base6b}^{\sage{factor6b}} $$

$ x = \answer[tolerance=0.05]{\sage{solution6}} $
\end{question}

% Q7
\begin{question}
Solve the exponential equation below. 

$$ \left(\sage{base7a}\right)^{\sage{factor7a}} = \sage{base7b}^{\sage{factor7b}} $$

$ x = \answer[tolerance=0.05]{\sage{solution7}} $
\end{question}

% Q8
\begin{question}
Solve the exponential equation below. 

$$ \sage{base8a}^{\sage{factor8a}} = \sage{base8b}^{\sage{factor8b}} $$

$ x = \answer[tolerance=0.05]{\sage{solution8}} $
\end{question}

\begin{sagesilent}
x = var("x")

def maybeMakeNegative(natural):
    integer = natural*(-1)**ZZ.random_element(2)
    return integer 

def generateFactor():
    a0 = maybeMakeNegative(ZZ.random_element(2, 7))
    a1 = maybeMakeNegative(ZZ.random_element(2, 7))
    factor = a0*x + a1
    return factor 

def generateRelativelyPrimeBases():
    b0 = ZZ.random_element(2, 9)
    b1 = ZZ.random_element(2, 9)
    while gcd(b0, b1) > 1:
        b0 = ZZ.random_element(2, 9)
        b1 = ZZ.random_element(2, 9)
    return [b0, b1]
##########
factor9a = generateFactor()
factor9b = generateFactor()
base9a, base9b = generateRelativelyPrimeBases()
#
while len(solve(factor9a * ln(base9a) - factor9b * ln(base9b) == 0, x)) == 0: 
    factor9a = generateFactor()
    factor9b = generateFactor()
    base9a, base9b = generateRelativelyPrimeBases()
#
solution9 = round(float( solve(factor9a * ln(base9a) - factor9b * ln(base9b) == 0, x)[0].rhs() ), 3)
#####
#####
factor10a = generateFactor()
factor10b = generateFactor()
base10a = generateRelativelyPrimeBases()[0] ** ZZ.random_element(2, 4)
base10b = generateRelativelyPrimeBases()[1] ** ZZ.random_element(2, 4)
#
while len(solve(factor10a * ln(base10a) - factor10b * ln(base10b) == 0, x)) == 0:
    factor10a = generateFactor()
    factor10b = generateFactor()
    base10a = generateRelativelyPrimeBases()[0] ** ZZ.random_element(2, 4)
    base10b = generateRelativelyPrimeBases()[1] ** ZZ.random_element(2, 4)
#
solution10 = round(float( solve(factor10a * ln(base10a) - factor10b * ln(base10b) == 0, x)[0].rhs() ), 3)
#####
#####
factor11a = generateFactor()
factor11b = generateFactor()
base11a = generateRelativelyPrimeBases()[0] ** ZZ.random_element(2, 4)
base11b = generateRelativelyPrimeBases()[1] ** - ZZ.random_element(2, 4)
#
while len(solve(factor11a * ln(base11a) - factor11b * ln(base11b) == 0, x)) == 0:
    factor11a = generateFactor()
    factor11b = generateFactor()
    base11a = generateRelativelyPrimeBases()[0] ** ZZ.random_element(2, 4)
    base11b = generateRelativelyPrimeBases()[1] ** - ZZ.random_element(2, 4)
#
solution11 = round(float( solve(factor11a * ln(base11a) - factor11b * ln(base11b) == 0, x)[0].rhs() ), 3)
\end{sagesilent}

% Q9
\begin{question}
Solve the exponential equation below. 

$$ \sage{base9a}^{\sage{factor9a}} = \sage{base9b}^{\sage{factor9b}} $$

$ x = \answer[tolerance=0.05]{\sage{solution9}} $
\end{question}

% Q10
\begin{question}
Solve the exponential equation below. 

$$ \sage{base10a}^{\sage{factor10a}} = \sage{base10b}^{\sage{factor10b}} $$

$ x = \answer[tolerance=0.05]{\sage{solution10}} $
\end{question}

% Q11
\begin{question}
Solve the exponential equation below. 

$$ \sage{base11a}^{\sage{factor11a}} = \sage{base11b}^{\sage{factor11b}} $$

$ x = \answer[tolerance=0.05]{\sage{solution11}} $
\end{question}

\begin{question}
\textbf{Main takeaway:} Before looking, you should work through the previous problems. \textit{Have you finished working through the examples?} $\answer[format=string]{Yes}$
\begin{feedback}[correct]
While changing the bases to be the same to rewrite the question can be easier sometimes, taking the log of both sides will \textbf{always} solve exponential equations.
\end{feedback}
\end{question}

\end{document}
